ROOT
@@ -1,0 +1,8 @@
+session CFG = Main +
+sessions
+  "HOL-Library"
+  "Regular-Sets"
+theories
+  CFG
+  CFL
+  Parse_Tree
